update `Theorems.v`

Theorems.v
@@ -72,6 +72,23 @@ Proof.
   auto.
 Qed.
 
+Lemma wf_typ'_weakening : forall T E F G,
+  wf_typ' (G ++ E) T ->
+  uniq (G ++ F ++ E) ->
+  wf_typ' (G ++ F ++ E) T.
+Proof.
+  intros.
+  remember (G ++ E) as F'.
+  generalize dependent G.
+  induction H; intros; subst; eauto.
+  pick fresh Y excluding (L `union` dom E `union` dom F `union` dom G) and apply wf_typ'_all; auto.
+  - apply wf_typ_weakening; auto.
+  - rewrite_env ((Y ~ T1 ++ G) ++ F ++ E).
+    apply H1; auto.
+    simpl_env.
+    auto.
+Qed.
+
 Lemma uniq_from_wf_env : forall E,
   wf_env E ->
   uniq E.
@@ -109,11 +126,148 @@ Proof.
   apply type_from_wf_typ with (E := E); auto.
 Qed.
 
+Fixpoint fv_tt (T : typ) {struct T} : atoms :=
+  match T with
+  | typ_top => {}
+  | typ_bvar J => {}
+  | typ_fvar X => {{ X }}
+  | typ_arrow T1 T2 => (fv_tt T1) `union` (fv_tt T2)
+  | typ_all T1 T2 => (fv_tt T1) `union` (fv_tt T2)
+  end.
+
+Fixpoint subst_tt (Z : atom) (U : typ) (T : typ) {struct T} : typ :=
+  match T with
+  | typ_top => typ_top
+  | typ_bvar J => typ_bvar J
+  | typ_fvar X => if X == Z then U else T
+  | typ_arrow T1 T2 => typ_arrow (subst_tt Z U T1) (subst_tt Z U T2)
+  | typ_all T1 T2 => typ_all (subst_tt Z U T1) (subst_tt Z U T2)
+  end.
+
+Lemma subst_tt_intro_rec : forall X T2 U k,
+  X `notin` fv_tt T2 ->
+  open_tt_rec k U T2 = subst_tt X U (open_tt_rec k (typ_fvar X) T2).
+Proof with congruence || auto.
+  induction T2; intros U k Fr; simpl in *; f_equal...
+  - destruct (k === n)... simpl. destruct (X == X)...
+  - destruct (a == X)... contradict Fr; fsetdec.
+Qed.
+
+Lemma subst_tt_intro : forall X T2 U,
+  X `notin` fv_tt T2 ->
+  open_tt T2 U = subst_tt X U (open_tt T2 X).
+Proof with auto.
+  intros.
+  unfold open_tt.
+  apply subst_tt_intro_rec...
+Qed.
+
+Lemma open_tt_rec_type_aux : forall T j V i U,
+  i <> j ->
+  open_tt_rec j V T = open_tt_rec i U (open_tt_rec j V T) ->
+  T = open_tt_rec i U T.
+Proof with congruence || eauto.
+  induction T; intros j V i U Neq H; simpl in *; inversion H; f_equal...
+  - destruct (j === n)... destruct (i === n)...
+Qed.
+
+Lemma open_tt_rec_type : forall T U k,
+  type T ->
+  T = open_tt_rec k U T.
+Proof with auto.
+  intros T U k Htyp. revert k.
+  induction Htyp; intros k; simpl; f_equal...
+  - unfold open_tt in *.
+    pick fresh X.
+    apply (open_tt_rec_type_aux T2 0 (typ_fvar X))...
+Qed.
+
+Lemma subst_tt_open_tt_rec : forall T1 T2 X P k,
+  type P ->
+  subst_tt X P (open_tt_rec k T2 T1) =
+    open_tt_rec k (subst_tt X P T2) (subst_tt X P T1).
+Proof with auto.
+  intros T1 T2 X P k WP. revert k.
+  induction T1; intros k; simpl; f_equal...
+  - destruct (k === n); subst...
+  - destruct (a == X); subst... apply open_tt_rec_type...
+Qed.
+
+Lemma subst_tt_open_tt_var : forall (X Y:atom) P T,
+  Y <> X ->
+  type P ->
+  open_tt (subst_tt X P T) Y = subst_tt X P (open_tt T Y).
+Proof with congruence || auto.
+  intros X Y P T Neq Wu.
+  unfold open_tt.
+  rewrite subst_tt_open_tt_rec...
+  simpl.
+  destruct (Y == X)...
+Qed.
+
+Lemma wf_typ_subst_tt : forall F Q E Z P T,
+  wf_typ (F ++ Z ~ Q ++ E) T ->
+  wf_typ E P ->
+  uniq (map (subst_tt Z P) F ++ E) ->
+  wf_typ (map (subst_tt Z P) F ++ E) (subst_tt Z P T).
+Proof with simpl_env; eauto using type_from_wf_typ'.
+  intros F Q E Z P T WT WP.
+  remember (F ++ Z ~ Q ++ E) as G.
+  generalize dependent F.
+  induction WT; intros F EQ Ok; subst; simpl subst_tt...
+  - destruct (X == Z); subst...
+    + rewrite_env (nil ++ map (subst_tt Z P) F ++ E).
+      apply wf_typ_weakening; auto.
+    + analyze_binds H...
+  - pick fresh Y excluding (L `union` singleton Z `union` dom E `union` dom F) and apply wf_typ_all...
+    rewrite subst_tt_open_tt_var...
+    rewrite_env (map (subst_tt Z P) (Y ~ T1 ++ F) ++ E).
+    apply H0...
+Qed.
+
+
+Lemma wf_typ'_subst_tt : forall F Q E Z P T,
+  wf_typ' (F ++ Z ~ Q ++ E) T ->
+  wf_typ E P ->
+  uniq (map (subst_tt Z P) F ++ E) ->
+  wf_typ' (map (subst_tt Z P) F ++ E) (subst_tt Z P T).
+Proof with simpl_env; eauto using type_from_wf_typ'.
+  intros F Q E Z P T WT WP.
+  remember (F ++ Z ~ Q ++ E) as G.
+  generalize dependent F.
+  induction WT; intros F EQ Ok; subst; simpl subst_tt...
+  - destruct (X == Z); subst...
+    + rewrite_env (nil ++ map (subst_tt Z P) F ++ E).
+      apply wf_typ'_weakening; auto.
+    + analyze_binds H...
+  - pick fresh Y excluding (L `union` singleton Z `union` dom E `union` dom F) and apply wf_typ'_all...
+    + eapply wf_typ_subst_tt; eauto.
+    + rewrite subst_tt_open_tt_var...
+      rewrite_env (map (subst_tt Z P) (Y ~ T1 ++ F) ++ E).
+      apply H1...
+Qed.
+
 Lemma wf_typ'_open : forall E U T1 T2,
-  uniq E ->
+  wf_env E ->
   wf_typ' E (typ_all T1 T2) ->
-  wf_typ' E U ->
+  wf_typ E U ->
   wf_typ' E (open_tt T2 U).
+Proof.
+  intros.
+  inversion H0; subst.
+  pick fresh Y for (L `union` fv_tt T2).
+  rewrite (subst_tt_intro Y); auto.
+  rewrite_env (map (subst_tt Y U) nil ++ E).
+  eapply wf_typ'_subst_tt; eauto.
+  simpl_env.
+  apply uniq_from_wf_env; auto.
+Qed.
+
+Lemma sub_narrowing_aux : forall Q F E Z P S T,
+  (forall E S T, wf_env E -> wf_typ' E Q -> wf_typ' E S -> sub E S Q -> wf_typ' E T -> sub E Q T -> sub E S T) ->
+  sub (F ++ Z ~ Q ++ E) S T ->
+  sub E P Q ->
+  sub (F ++ Z ~ P ++ E) S T.
 Admitted.
 
 Theorem sub_transitivity :
@@ -168,7 +322,7 @@ Proof.
       apply wf_typ'_from_wf_typ.
       apply wf_typ_from_binds_typ with (X := X); auto.
     + inversion Heq; inversion QsubT; subst; auto.
-      pick fresh Y excluding (L `union` dom E) and apply sub_all.
+      pick fresh Y excluding (L `union` dom E `union` fv_tt T4 `union` L0 `union` L1) and apply sub_all.
       * apply IHW with (Q' := T1); auto.
         -- inversion HwfQ; auto.
         -- inversion HwfT; auto.
@@ -176,45 +330,33 @@ Proof.
       * apply H0 with (X := Y) (Q' := open_tt T2 Y); auto.
         -- apply wf_env_sub; auto.
            inversion HwfT; auto.
-        -- apply wf_typ'_open with (T1 := T1).
-           ++ apply uniq_from_wf_env; auto.
+        -- apply wf_typ'_open with (T1 := T1) (U := Y); auto.
+           ++ inversion HwfT; auto.
+           ++ rewrite_env (nil ++ Y ~ T4 ++ E).
+              apply wf_typ'_weakening; auto.
+              simpl_env.
+              apply uniq_from_wf_env.
               apply wf_env_sub; auto.
               inversion HwfT; auto.
-           ++ apply wf_typ'_all with (L := dom (Y ~ T4 ++ E)).
-              ** rewrite_env (nil ++ Y ~ T4 ++ E).
-                 apply wf_typ_weakening; simpl_env.
-                 --- inversion HwfQ; auto.
-                 --- apply uniq_from_wf_env.
-                     apply wf_env_sub; auto.
-                     inversion HwfT; auto.
-              ** admit.
-           ++ apply wf_typ'_var with (U := T4); auto.
-        -- apply wf_typ'_open with (T1 := S1).
-           ++ apply uniq_from_wf_env; auto.
+           ++ apply wf_typ_var with (U := T4); auto.
+        -- apply wf_typ'_open with (T1 := S1) (U := Y); auto.
+           ++ inversion HwfT; auto.
+           ++ rewrite_env (nil ++ Y ~ T4 ++ E).
+              apply wf_typ'_weakening; auto.
+              simpl_env.
+              apply uniq_from_wf_env.
               apply wf_env_sub; auto.
               inversion HwfT; auto.
-           ++ apply wf_typ'_all with (L := dom (Y ~ T4 ++ E)).
-              ** rewrite_env (nil ++ Y ~ T4 ++ E).
-                 apply wf_typ_weakening; simpl_env.
-                 --- inversion HwfS; auto.
-                 --- apply uniq_from_wf_env.
-                     apply wf_env_sub; auto.
-                     inversion HwfT; auto.
-              ** intros. admit.
-           ++ apply wf_typ'_var with (U := T4); auto.
-        -- admit.
-        -- apply wf_typ'_open with (T1 := T4).
-           ++ apply uniq_from_wf_env; auto.
+           ++ apply wf_typ_var with (U := T4); auto.
+        -- rewrite_env (nil ++ Y ~ T4 ++ E).
+           apply sub_narrowing_aux with (Q := T1); eauto.
+        -- apply wf_typ'_open with (T1 := T4) (U := Y); auto.
+           ++ inversion HwfT; auto.
+           ++ rewrite_env (nil ++ Y ~ T4 ++ E).
+              apply wf_typ'_weakening; auto.
+              simpl_env.
+              apply uniq_from_wf_env.
               apply wf_env_sub; auto.
               inversion HwfT; auto.
-           ++ apply wf_typ'_all with (L := dom (Y ~ T4 ++ E)).
-              ** rewrite_env (nil ++ Y ~ T4 ++ E).
-                 apply wf_typ_weakening; simpl_env.
-                 --- inversion HwfT; auto.
-                 --- apply uniq_from_wf_env.
-                     apply wf_env_sub; auto.
-                     inversion HwfT; auto.
-              ** intros. admit.
-           ++ apply wf_typ'_var with (U := T4); auto.
-        -- admit.
-Admitted.
+           ++ apply wf_typ_var with (U := T4); auto.
+Qed.
